@prefix owl: <http://www.w3.org/2002/07/owl#> .
@prefix rdf: <http://www.w3.org/1999/02/22-rdf-syntax-ns#> .
@prefix rdfs: <http://www.w3.org/2000/01/rdf-schema#> .
@prefix xsd:  <http://www.w3.org/2001/XMLSchema#> .
@prefix dct: <http://purl.org/dc/terms/> .
@prefix ssn: <http://purl.oclc.org/NET/ssnx/ssn> .
@prefix mto: <http://example.org/mto/mtconnectmachinedata#> .
@prefix vann: <http://purl.org/vocab/vann/> .
@prefix part: <http://www.w3.org/2001/sw/BestPractices/OEP/SimplePartWhole/part.owl#>.
@prefix saref: <https://w3id.org/c>.

# Description of this ontology
# ----------------------------

mto:
	 rdf:type owl:Ontology;
   	 dct:title "MTConnect Ontology"@en;
     rdfs:comment "Ontology developed based on MTConnect standard.";
     dct:creator "Glykeria Alvanou" ;
     dct:created "2017-06-05"^^xsd:date;
     dct:modified "2018-02-09"^^xsd:date;
     vann:preferredNamespacePrefix "mto".

##### CLASSES #####

mto:Device 
		rdf:type owl:Class;
		owl:equivalentClass ssn:Device;
		rdfs:label "Device"^^xsd:string;
		rdfs:comment "Represents a single piece of equipment (i.e. machine) or any logical grouping of pieces of equipment that operate together to perform a function.";
		rdf:type         owl:Restriction ; 
		owl:onProperty   mto:hasUuid, mto:hasId, saref:hasName;
		owl:cardinality  "1"^^xsd:nonNegativeInteger.
     	       
mto:Component 
		rdf:type owl:Class;
		rdfs:label "Component"^^xsd:string;
		rdfs:comment "Defines the structure of the physical or logical parts of a device that provide more precise definition for the structure of the device.";
		rdf:type         owl:Restriction ; 
		owl:onProperty   mto:hasId;
		owl:cardinality  "1"^^xsd:nonNegativeInteger.

##Component types
mto:Actuator
		rdf:type owl:Class;
		rdfs:subClassOf mto:Component;
		rdfs:label "Actuator"^^xsd:string;
		rdfs:comment "Describes a device for moving or controlling a mechanism or system.".

mto:Axe 
		rdf:type owl:Class;
		rdfs:subClassOf mto:Component;
		rdfs:label "Axe"^^xsd:string;
		rdfs:comment "Performs linear or rotational motion associated with a device.";
		rdf:type         owl:Restriction ; 
		owl:onProperty   ssn:hasSubSystem ;
		owl:onClass      mto:LinearAxe, mto:RotaryAxe;
		owl:mincardinality  "1"^^xsd:nonNegativeInteger.

mto:Controller 
		rdf:type owl:Class;
		rdfs:subClassOf mto:Component;
		rdfs:label "Controller"^^xsd:string;
		rdfs:comment "The intelligent or computational part of a device which monitors and calculated information.".

mto:Door 
		rdf:type owl:Class;
		rdfs:subClassOf mto:Component;
		rdfs:label "Door"^^xsd:string;
		rdfs:comment "Mechanisms or closures that can cover access portals into a device.";
		owl:onProperty   mto:hasDataItem ;
		owl:onClass      mto:DoorState;
		owl:mincardinality  "1"^^xsd:nonNegativeInteger.

mto:Interface 
		rdf:type owl:Class;
		rdfs:subClassOf mto:Component;
		rdfs:comment "The information used to coordinate actions and activity between devices or sub-systems and a device.".

mto:Sensor 
		rdf:type owl:Class;
		rdfs:subClassOf mto:Component;
		rdfs:label "Sensor"^^xsd:string;
		rdfs:comment "Represents a measurement device.".

mto:Stock 
		rdf:type owl:Class;
		rdfs:subClassOf mto:Component;
		rdfs:label "Stock"^^xsd:string;
		rdfs:comment "The material to which work is applied in a machine or piece of equipment to produce parts.".

mto:System 
		rdf:type owl:Class;
		rdfs:subClassOf mto:Component;
		rdfs:label "System"^^xsd:string;
		rdfs:comment "Describe the major sub-systems that provide services to a device.".


##Subcomponent types

mto:Coolant 
		rdf:type owl:Class;
		rdfs:subClassOf mto:System;
		rdfs:label "Coolant"^^xsd:string;
		rdfs:comment "Coolant represents a system comprised of all the parts involved in distribution and management of fluids that remove heat from a piece of equipment.".

mto:Electric
		rdf:type owl:Class;
		rdfs:subClassOf mto:System;
		rdfs:label "Electric"^^xsd:string;
		rdfs:comment "Electric represents the main power supply or generator for the device.".

mto:Hydraulic
		rdf:type owl:Class;
		rdfs:subClassOf mto:System;
		rdfs:label "Hydraulic"^^xsd:string;
		rdfs:comment "Hydraulic represents a system comprised of all the parts involved in moving and distributing pressurized liquid for the purpose of delivering a source of power to specific types of actuators.".
	
mto:LinearAxe
		rdf:type owl:Class;
		rdfs:subClassOf mto:Axe;
		rdfs:label "LinearAxe"^^xsd:string;
		rdfs:comment "Represents the movement of a physical device, or a portion of a device in a straight line.".

mto:Lubrication 
		rdf:type owl:Class;
		rdfs:subClassOf mto:System;
		rdfs:label "Lubrication"^^xsd:string;
		rdfs:comment "Lubrication represents a system comprised of all the parts involved in distribution and management of fluids used to lubricate parts of the piece of the equipment.".

mto:RotaryAxe #a rotary axis MUST specify a subType attribute of SPINDLE, INDEX, or CONTOUR.
		rdf:type owl:Class;
		rdfs:subClassOf mto:Axe;
		rdfs:label "RotaryAxe"^^xsd:string;
		rdfs:comment "Represents any non-linear or rotary movement of a physical device or a portion of a device.".

mto:Path 
		rdf:type owl:Class;
		rdfs:subClassOf mto:Controller;
		rdfs:label "Path"^^xsd:string;
		rdfs:comment "Represents the information for an independent operation or function within a controller.".

mto:Pneumatic 
		rdf:type owl:Class;
		rdfs:subClassOf mto:System;
		rdfs:label "Pneumatic"^^xsd:string;
		rdfs:comment "Represents a system comprised of all the parts involved in moving and distributing pressurized gas regardless of purpose or activity.".


#OTHER CLASSES
ssn:Device 			rdf:type owl:Class;
					rdfs:label "Device"^^xsd:string;
					rdfs:isDefinedBy ssn: ;
					rdfs:comment "A device is a physical piece of technology - a system in a box. Devices may of course be built of smaller devices and software components (i.e. 
systems have components).".

mto:Chuck 
		rdf:type owl:Class;
		rdfs:label "Chuck"^^xsd:string;
		rdfs:comment "Represents a mechanism that holds a part or stock material in place.".

mto:Acceleration rdf:type owl:Class;
					rdfs:subClassOf mto:DataItem;
					rdfs:label "Acceleration"^^xsd:string;
					rdfs:comment "Rate of change of velocity.".

mto:AccumulatedTime rdf:type owl:Class;
					rdfs:subClassOf mto:DataItem;
					rdfs:label "AccumulatedTime"^^xsd:string;
					rdfs:comment "The measurement of accumulated time for an activity or event.".

mto:ActuatorCondition rdf:type owl:Class;
					rdfs:subClassOf mto:DataItem;
					rdfs:label "ActuatorCondition"^^xsd:string;
					rdfs:comment "An actuator’s status.".

mto:AngularVelocity rdf:type owl:Class;
					rdfs:subClassOf mto:DataItem;
					rdfs:label "AngularVelocity"^^xsd:string;
		        	rdfs:comment "Rate of change of angular position.".

mto:Angle rdf:type owl:Class;
		  rdfs:subClassOf mto:DataItem;
		  rdfs:label "Angle"^^xsd:string;
		  rdfs:comment "The measurement of angular position.".

mto:AssetChanged rdf:type owl:Class;
		  rdfs:subClassOf mto:DataItem;
		  rdfs:label "AssetChanged"^^xsd:string.

mto:AssetRemoved rdf:type owl:Class;
		  rdfs:subClassOf mto:DataItem;
		  rdfs:label "AssetRemoved"^^xsd:string.

mto:Availability rdf:type owl:Class;
				 rdfs:comment "Represents the ability of a Structural Element to communicate.";
				 rdfs:subClassOf mto:DataItem;
				 rdfs:label "Availability"^^xsd:string;
				 owl:oneOf (
							"AVAILABLE" "UNAVAILABLE" ).

mto:AxisFeedrate rdf:type owl:Class;
		  rdfs:subClassOf mto:DataItem;
		  rdfs:label "AxisFeedrate"^^xsd:string;
		  rdfs:comment "The feedrate of a linear axis.".

mto:AxisFeedrateOverride rdf:type owl:Class;
		 				 rdfs:subClassOf mto:DataItem;
		 				 rdfs:label "AxisFeedrateOverride"^^xsd:string;
		 				 rdfs:comment "The value of a signal or calculation issued to adjust the feedrate of an individual linear type axis.".

mto:ChuckInterlock rdf:type owl:Class;
		  rdfs:subClassOf mto:DataItem;
		  rdfs:label "ChuckInterlock"^^xsd:string;
		  rdfs:comment "An indication of the operational condition of the interlock function for an electronically controller chuck.".

mto:ChuckState rdf:type owl:Class;
				rdfs:subClassOf mto:DataItem;
				rdfs:label "ChuckState"^^xsd:string;
		owl:oneOf (
			"OPEN" "CLOSED" "UNLATCHED" ).

mto:Communication rdf:type owl:Class;
		  rdfs:subClassOf mto:DataItem;
		  rdfs:label "Communication"^^xsd:string;
		  rdfs:comment "A communications failure indicator.".

mto:Condition rdf:type owl:Class;
			 # rdfs:subClassOf mto:DataItemCategory;
			  rdfs:label "Condition"^^xsd:string;
			  rdfs:comment "A CONDITION communicates information about the health of a device and its ability to function";
			  owl:oneOf (
							"NORMAL" "WARNING" "FAULT" "UNAVAILABLE"  ).

mto:ControllerMode  rdf:type owl:Class;
					rdfs:subClassOf mto:DataItem;
					rdfs:label "ControllerMode"^^xsd:string;
					rdfs:comment "The current mode of the Controller.";
				    owl:oneOf (
			                 "AUTOMATIC" "MANUAL" "MANUAL_DATA_INPUT" "SEMI_AUTOMATIC" "EDIT").

mto:DataItem 
		rdf:type owl:Class;
		rdfs:label "DataItem"^^xsd:string;
		rdfs:comment "DataItem provides a detailed description for each piece of data that is collected from a device.";
		rdf:type         owl:Restriction ; 
		owl:onProperty   mto:hasId, mto:hasCategory;
		owl:cardinality  "1"^^xsd:nonNegativeInteger.

#mto:DataItemCategory rdf:type owl:Class.

#mto:DataItemSubType rdf:type owl:Class;
	#	owl:oneOf (
	#		"ACTUAL" "COMMANDED" ).

mto:DataRange rdf:type owl:Class;
		  rdfs:subClassOf mto:DataItem;
		  rdfs:label "DataRange"^^xsd:string;
		  rdfs:comment "Information provided is outside of expected value range.".

mto:Direction rdf:type owl:Class;
		  rdfs:subClassOf mto:DataItem;
		  rdfs:label "Direction"^^xsd:string;
		  rdfs:comment "The direction of motion.".

mto:DirectionCondition rdf:type owl:Class;
		  rdfs:subClassOf mto:DataItem;
		  rdfs:label "DirectionCondition"^^xsd:string;
		  rdfs:comment "An indication of a fault associated with the direction of motion of a Structural Element.".

mto:DoorState rdf:type owl:Class;
				rdfs:subClassOf mto:DataItem;
				rdfs:label "DoorState"^^xsd:string;
		owl:oneOf (
			"OPEN" "CLOSED" "UNLATCHED" ).

mto:EmergencyStop rdf:type owl:Class;
				  rdfs:subClassOf mto:DataItem;
				  rdfs:label "EmergencyStop"^^xsd:string;
				  owl:oneOf (
					"ARMED" "TRIGGERED" );
				  rdfs:comment "The current state of the emergency stop signal for a machine, device, controller path, or any other component or subsystem of a device".

mto:EndOfBar rdf:type owl:Class;
		  rdfs:subClassOf mto:DataItem;
		  rdfs:label "EndOfBar"^^xsd:string;
		  owl:oneOf (
			"YES" "NO" );
		  rdfs:comment "An indication that the end of a piece of bar stock has been reached.".

#mto:Event rdf:type owl:Class;
#		   rdfs:subClassOf mto:DataItemCategory;
#		   rdfs:label "Event"^^xsd:string;
#		   rdfs:comment "An EVENT is a data value representing a discrete piece of information from the device. The data provided may be a numeric value or text".

mto:Execution   rdf:type owl:Class;
				rdfs:subClassOf mto:DataItem;
				rdfs:label "Execution"^^xsd:string;
				rdfs:comment "The execution status of the Controller.";
				owl:oneOf (
			                "READY" "ACTIVE" "INTERRUPTED" "FEED_HOLD" "STOPPED" "OPTIONAL_STOP" "PROGRAM_STOPPED" "PROGRAM_COMPLETED" ).

mto:FunctionalMode rdf:type owl:Class;
					rdfs:subClassOf mto:DataItem;
					rdfs:label "FunctionalMode"^^xsd:string;
					rdfs:comment "The current intended production status of the device or component.";
		owl:oneOf (
			"PRODUCTION" "SETUP" "TEARDOWN" "MAINTENANCE" "PROCESS DEVELOPMENT" ).

mto:Hardware rdf:type owl:Class;
		  rdfs:subClassOf mto:DataItem;
		  rdfs:label "Hardware"^^xsd:string;
		  rdfs:comment "The hardware subsystem of the Structural Element’s operation condition.".

mto:InterfaceState rdf:type owl:Class;
		  rdfs:subClassOf mto:DataItem;
		  rdfs:label "InterfaceState"^^xsd:string;
		  owl:oneOf (
			"ENABLED" "DISABLED" );
		  rdfs:comment "An indication of the operation condition of an Interface.".

mto:Level rdf:type owl:Class;
		  rdfs:subClassOf mto:DataItem;
		  rdfs:label "Level"^^xsd:string;
		  rdfs:comment "The measurement of the amount of a substance remaining compared to the planned maximum amount of that substance.".

mto:Line rdf:type owl:Class;
		  rdfs:subClassOf mto:DataItem;
		  rdfs:label "Line"^^xsd:string;
		  rdfs:comment "The current line of code being executed.".

mto:Load rdf:type owl:Class;
		  rdfs:subClassOf mto:DataItem;
		  rdfs:label "Load"^^xsd:string;
		  rdfs:comment "The measurement of the actual versus the standard rating of a device.".

mto:LogicProgram rdf:type owl:Class;
		  rdfs:subClassOf mto:DataItem;
		  rdfs:label "LogicProgram"^^xsd:string;
		  rdfs:comment "An error occurred in the logic program or PLC (programmable logic controller)".

mto:MotionProgram rdf:type owl:Class;
		  rdfs:subClassOf mto:DataItem;
		  rdfs:label "MotionProgram"^^xsd:string;
		  rdfs:comment "An error occurred in the motion program.".

mto:PalletId rdf:type owl:Class;
		  rdfs:subClassOf mto:DataItem;
		  rdfs:label "PalletId"^^xsd:string;
		  rdfs:comment "The identifier for the pallet currently in use.".

mto:PalletNumber rdf:type owl:Class;
		  		 rdfs:subClassOf mto:DataItem;
		  		 rdfs:label "PalletId"^^xsd:string;
		 		 rdfs:comment "The identifier for the pallet currently in use.".

mto:PartCount rdf:type owl:Class;
		  rdfs:subClassOf mto:DataItem;
		  rdfs:label "PartCount"^^xsd:string;
		  rdfs:comment "The current count of parts produced as represented by the Controller.".	

mto:PathFeedrate rdf:type owl:Class;
		  rdfs:subClassOf mto:DataItem;
		  rdfs:label "PathFeedrate"^^xsd:string;
		  rdfs:comment "The feedrate for the axes associated with a Path component - may represent a single axis or the coordinated movement of multiple axes – a vector.".

mto:PathFeedrateOverride rdf:type owl:Class;
		  rdfs:subClassOf mto:DataItem;
		  rdfs:label "PathFeedrateOverride"^^xsd:string;
		  rdfs:comment "The value of a signal or calculation issued to adjust the feedrate for the axes associated with a Path component.".

mto:PathPosition rdf:type owl:Class;
		  		 rdfs:subClassOf mto:DataItem;
		  		 rdfs:label "PathPosition"^^xsd:string;
		  		 rdfs:comment "The current program control point expressed in WORK coordinates.".

mto:Pressure rdf:type owl:Class;
		  	 rdfs:subClassOf mto:DataItem;
		  	 rdfs:label "Pressure"^^xsd:string;
		  	 rdfs:comment "The force per unit area exerted by a gas or liquid.".

mto:Program rdf:type owl:Class;
		  rdfs:subClassOf mto:DataItem;
		  rdfs:label "Program"^^xsd:string;
		  rdfs:comment "The name of the program being executed by the Controller component.".

mto:ProgramComment rdf:type owl:Class;
		  rdfs:subClassOf mto:DataItem;
		  rdfs:label "ProgramComment"^^xsd:string;
		  rdfs:comment "A comment or non-executable statement in the control program.".

mto:ProgramEdit rdf:type owl:Class;
				rdfs:subClassOf mto:DataItem;
				rdfs:label "ProgramEdit"^^xsd:string;
				rdfs:comment "An indication of the Controller component’s program editing mode.";
		owl:oneOf (
			"ACTIVE" "READY" "NOT_READY" "UNAVAILABLE" ).

mto:ProgramEditName rdf:type owl:Class;
		  			rdfs:subClassOf mto:DataItem;
		 			rdfs:label "ProgramEditName"^^xsd:string;
		  			rdfs:comment "The name of the program being edited.".

mto:Position rdf:type owl:Class;
		  rdfs:subClassOf mto:DataItem;
		  rdfs:label "Position"^^xsd:string;
		  rdfs:comment "The position of the component.".

mto:PowerState  rdf:type owl:Class;
				rdfs:subClassOf mto:DataItem;
				rdfs:label "PowerState"^^xsd:string;
				rdfs:comment "The indication of the status of the source of energy for a Structural Element to allow it to perform its intended function and the state of an enabling signal providing permission for the Structural Element to perform its functions.";
				owl:oneOf (
									"ON" "OFF" "UNAVAILABLE" ).

mto:RotaryMode rdf:type owl:Class;
		  rdfs:subClassOf mto:DataItem;
		  rdfs:label "RotaryMode"^^xsd:string;
		  owl:oneOf (
			"SPINDLE" "INDEX" "CONTOUR");
		  rdfs:comment "The mode for a Rotary type axis.".

mto:RotaryVelocity rdf:type owl:Class;
		  		   rdfs:subClassOf mto:DataItem;
		  		   rdfs:label "RotaryVelocity"^^xsd:string;
		  		   rdfs:comment "The rotational speed of a rotary axis.".

mto:RotaryVelocityOverride rdf:type owl:Class;
		  				   rdfs:subClassOf mto:DataItem;
		  			       rdfs:label "RotaryVelocityOverride"^^xsd:string;
		  				   rdfs:comment "A command issued to adjust the programmed velocity for a Rotary type axis.".

#mto:Sample rdf:type owl:Class;
		 #  rdfs:subClassOf mto:DataItemCategory;
		 #  rdfs:label "Sample"^^xsd:string;
		 #  rdfs:comment "A SAMPLE is the reading of the value of a continuously variable or analog data value".

mto:SequenceNumber rdf:type owl:Class;
		  			rdfs:subClassOf mto:DataItem;
		  			rdfs:label "SequenceNumber"^^xsd:string.

mto:SystemCondition rdf:type owl:Class;
		  			rdfs:subClassOf mto:DataItem;
		  			rdfs:label "SystemCondition"^^xsd:string;
		  			rdfs:comment "A CONDITION representing something that is not the operator, program, or hardware.".

mto:Temperature rdf:type owl:Class;
		  rdfs:subClassOf mto:DataItem;
		  rdfs:label "Temperature"^^xsd:string;
		  rdfs:comment "The measurement of temperature.".

mto:ToolAssetId rdf:type owl:Class;
		  rdfs:subClassOf mto:DataItem;
		  rdfs:label "ToolAssetId"^^xsd:string;
		  rdfs:comment "The identifier of an individual tool asset which is the current tool in use by a piece of equipment.".

mto:ToolGroup rdf:type owl:Class;
		  rdfs:subClassOf mto:DataItem;
		  rdfs:label "ToolGroup"^^xsd:string.

mto:ToolNumber rdf:type owl:Class;
		  rdfs:subClassOf mto:DataItem;
		  rdfs:label "ToolNumber"^^xsd:string;
		  rdfs:comment "The identifier assigned by the Controller component to the current tool in use by a piece of equipment.".

mto:ToolSuffix rdf:type owl:Class;
		  rdfs:subClassOf mto:DataItem;
		  rdfs:label "ToolSuffix"^^xsd:string.

mto:Torque rdf:type owl:Class;
		  rdfs:subClassOf mto:DataItem;
		  rdfs:label "Torque"^^xsd:string;
		  rdfs:comment "The turning force exerted on an object or by an object.".	

mto:Velocity rdf:type owl:Class;
		  rdfs:subClassOf mto:DataItem;
		  rdfs:label "Velocity"^^xsd:string;
		  rdfs:comment "The rate of change of position.".

mto:Voltage rdf:type owl:Class;
		  rdfs:subClassOf mto:DataItem;
		  rdfs:label "Voltage"^^xsd:string;
		  rdfs:comment "The measurement of electrical potential between two points.".

mto:xMotion rdf:type owl:Class;
		  rdfs:subClassOf mto:DataItem;
		  rdfs:label "xMotion"^^xsd:string.

mto:xUnit rdf:type owl:Class;
		  rdfs:subClassOf mto:DataItem;
		  rdfs:label "xUnit"^^xsd:string.

#### PROPERTIES ####

#### Object Properties ####

mto:hasAvailability				
				rdf:type 	    owl:ObjectProperty;
		      	rdfs:domain 	mto:DataItem; #ssn:Device, mto:Component
		      	rdfs:range 		mto:Availability. 

mto:hasCondition 
				rdf:type 	owl:ObjectProperty;
		      	rdfs:domain  mto:DataItem; #mto:Component; rdfs:range
		      	rdfs:range   mto:Condition.  	 

mto:hasControllerMode
				rdf:type 		owl:ObjectProperty;
		      	rdfs:domain 	mto:DataItem;
		      	rdfs:range 		mto:ControllerMode.

mto:hasDataItem
				rdf:type 	    owl:ObjectProperty;
		      	rdfs:domain 	mto:Device, mto:Component;
		      	rdfs:range 	    mto:DataItem.

mto:hasEmergencyStop
				rdf:type 	owl:ObjectProperty;
		      	rdfs:domain 	mto:DataItem;
		      	rdfs:range mto:EmergencyStop. #mto:Device, mto:Component; rdfs:range 	 
		      	
mto:hasExecution
				rdf:type 	owl:ObjectProperty;
		      	rdfs:domain  mto:DataItem; 	 
		      	rdfs:range mto:Execution.

mto:hasFunctionalMode				
				rdf:type 	owl:ObjectProperty;
		      	rdfs:domain mto:DataItem;
		      	rdfs:range mto:FunctionalMode.#	mto:Device, mto:Component; rdfs:range 	 


mto:hasProgramEdit
				rdf:type 	owl:ObjectProperty;
		      	rdfs:domain mto:DataItem;
		      	rdfs:range mto:ProgramEdit.#	mto:Controller; rdfs:range 	 
		      	
mto:hasPowerState	
				rdf:type 		owl:ObjectProperty;
		      	rdfs:domain 	mto:DataItem; #mto:Device, mto:Component;rdfs:range 	 
		      	rdfs:range  	mto:PowerState.

mto:hasChuckState	
				rdf:type 	owl:ObjectProperty;
		      	rdfs:domain 	mto:Chuck;
		      	rdfs:range 	mto:ChuckState.

#### Datatype Properties ####

mto:hasAccumulatedTime	 
				rdf:type 			owl:DatatypeProperty;
		      	rdfs:domain 		mto:AccumulatedTime;
		      	rdfs:range 	 		xsd:string.

mto:hasAngle 		
				rdf:type 			owl:DatatypeProperty;
		      	rdfs:domain 		mto:Angle; 
		      	rdfs:range 	 		rdfs:Literal.

mto:hasAngularVelocity 	
				rdf:type 					owl:DatatypeProperty;
				rdfs:subPropertyOf 			owl:hasValue;
		      	rdfs:domain 				mto:AngularVelocity; 
		      	rdfs:range 	 				rdfs:Literal.

mto:hasAxisFeedrate	
				rdf:type 		owl:DatatypeProperty;
		      	rdfs:domain 	mto:AxisFeedrate;
		      	rdfs:range 	 	rdfs:Literal.

mto:hasCategory 
				rdf:type 		owl:ObjectProperty;
		      	rdfs:domain 	mto:DataItem;
		      	rdfs:range 	 	xsd:string.

mto:hasConditionMessage
				rdf:type 		owl:DatatypeProperty;
		      	rdfs:domain 	mto:Condition;
		      	rdfs:range 	 	xsd:string.

mto:hasConfiguration
				rdf:type 		owl:DatatypeProperty;
		      	rdfs:domain 	mto:Sensor;
		      	rdfs:range 	 	xsd:string.

mto:hasCoordinateSystem
			rdf:type 		owl:DatatypeProperty;
			rdfs:domain 	mto:DataItem;
			rdfs:range 		xsd:string.

mto:hasCreationTime	
				rdf:type 			owl:DatatypeProperty;
		      	rdfs:domain 		mto:Device; 
		      	rdfs:range 	 		xsd:dateTime;
		      	rdfs:comment 		"The time the request was made.".
mto:hasId	
			rdf:type 		owl:DatatypeProperty;
			rdfs:domain 	mto:Device, mto:Component, mto:DataItem;
			rdfs:range 		xsd:string;
			rdfs:comment    "A unique identifier of a structural element.".

mto:hasLine		
				rdf:type 		owl:DatatypeProperty;
		      	rdfs:domain 	mto:Line;
		      	rdfs:range 	 	xsd:string.

mto:hasLoad 	
				rdf:type 		owl:DatatypeProperty;
		      	rdfs:domain 	mto:Load;
		      	rdfs:range 	 	rdfs:Literal.

#saref:hasName	
		#	rdf:type 	owl:DatatypeProperty;
		#	rdfs:domain 	ssn:Device, mto:Component, mto:DataItem;
		#	rdfs:range 		 xsd:string;
		#	rdfs:comment    "The name of the device or a component.";
		#	rdfs:label "has name".

mto:hasNativeScale	
			rdf:type 		owl:DatatypeProperty;
			rdfs:domain 	mto:DataItem;
			rdfs:range 		xsd:string.

mto:hasNativeUnits	
			rdf:type 		owl:DatatypeProperty;
			rdfs:domain 	mto:DataItem;
			rdfs:range 		xsd:string.

mto:hasPalletId
				rdf:type 		owl:DatatypeProperty ;
		      	rdfs:domain 	mto:PalletId ;
		      	rdfs:range		xsd:string.

mto:hasPalletNumber
				rdf:type 		owl:DatatypeProperty ;
		      	rdfs:domain 	mto:PalletNumber ;
		      	rdfs:range 		xsd:string.

#ssn:hasPart
			#rdf:type owl:TransitiveProperty;
			#rdfs:label "has part";
			#rdfs:comment "A schematic relation between any entities e.g. 'the human body has a brain as part".
			
mto:hasPartCount	
				rdf:type 		owl:DatatypeProperty;
		      	rdfs:domain 	mto:PartCount;
		      	rdfs:range 	 	rdfs:Literal.

mto:hasPathFeedrate	
				rdf:type 		owl:DatatypeProperty;
		      	rdfs:domain 	mto:PathFeedrate;
		      	rdfs:range 	 	xsd:string.

mto:hasPathFeedrateOverride	
				rdf:type 		owl:DatatypeProperty;
		      	rdfs:domain 	mto:PathFeedrateOverride;
		      	rdfs:range 	 	xsd:string.

mto:hasPathPosition	
				rdf:type 		owl:DatatypeProperty;
		      	rdfs:domain 	mto:Path;
		      	rdfs:range 	 	xsd:string.

mto:hasPosition	
				rdf:type 	    owl:DatatypeProperty;
		      	rdfs:domain 	mto:Position;
		      	rdfs:range 	    xsd:string.	

mto:hasPressure
				rdf:type 		owl:DatatypeProperty;
		      	rdfs:domain 	mto:Pressure;
		      	rdfs:range 	 	xsd:string.

mto:hasProgram
				rdf:type 		owl:DatatypeProperty;
		      	rdfs:domain 	mto:Controller;
		      	rdfs:range 	 	xsd:string.	

mto:hasProgramComment
				rdf:type 		owl:DatatypeProperty;
		      	rdfs:domain 	mto:ProgramComment;
		      	rdfs:range 	 	xsd:string.

mto:hasProgramEditName
				rdf:type 		owl:DatatypeProperty;
		      	rdfs:domain 	mto:ProgramEditName;
		      	rdfs:range 	 	xsd:string.

mto:hasRotaryMode
				rdf:type 		owl:DatatypeProperty;
		      	rdfs:domain 	mto:RotaryMode;
		      	rdfs:range 		xsd:string.

mto:hasRotaryVelocity 	
				rdf:type 		owl:DatatypeProperty;
		      	rdfs:domain 	mto:RotaryVelocity;
		      	rdfs:range 	 	xsd:string.	

mto:hasRotaryVelocityOverride
				rdf:type 		owl:DatatypeProperty;
		      	rdfs:domain 	mto:RotaryVelocityOverride;
		      	rdfs:range 	 	xsd:string.

mto:hasSampleRate	
			rdf:type 		owl:DatatypeProperty;
			rdfs:domain 	mto:DataItem;
			rdfs:range 		 xsd:string.

mto:hasSequence
			rdf:type 	owl:DatatypeProperty;
			rdfs:domain 	mto:DataItem;
		    rdfs:range xsd:integer.

mto:hasSequenceNumber
			rdf:type 		owl:DatatypeProperty;
			rdfs:domain 	mto:DataItem;
		    rdfs:range 		xsd:integer.

mto:hasSignificantDigits
			rdf:type 		owl:DatatypeProperty;
			rdfs:domain 	mto:DataItem;
			rdfs:range 		 xsd:string.

mto:hasSubType	
			rdf:type 		owl:DatatypeProperty;
			rdfs:domain 	mto:DataItem;
			rdfs:range      rdfs:string;
			rdfs:comment    "A sub-categorization of the data item type.".

mto:hasTemperature 	
				rdf:type 			owl:DatatypeProperty;
				rdfs:subPropertyOf  owl:hasValue;
		      	rdfs:domain   		mto:Temperature;
		      	rdfs:range 			xsd:string.

mto:hasToolAssetId 	
				rdf:type 	  owl:DatatypeProperty;
		      	rdfs:domain   mto:ToolAssetId;
		      	rdfs:range 	  xsd:string.

mto:hasToolGroup 	
				rdf:type 	  owl:DatatypeProperty;
		      	rdfs:domain   mto:ToolGroup;
		      	rdfs:range 	  xsd:string.

mto:hasToolNumber 	
				rdf:type 	  owl:DatatypeProperty;
		      	rdfs:domain   mto:ToolNumber;
		      	rdfs:range 	  xsd:string.

mto:hasToolSuffix 	
				rdf:type 	  owl:DatatypeProperty;
		      	rdfs:domain   mto:ToolSuffix;
		      	rdfs:range 	  xsd:string.
#mto:hasTimestamp	
		#		rdf:type 		owl:DatatypeProperty;
		#      	rdfs:domain  	mto:DataItem; 
		#      	rdfs:range 	 	xsd:dateTime;
		 #     	rdfs:comment 	"The time the data were reported.".	

mto:hasUnits	
			rdf:type 		owl:DatatypeProperty;
			rdfs:domain 	mto:DataItem;
			rdfs:range 		xsd:string.	

mto:hasUuid	
			rdf:type 		owl:DatatypeProperty;
			rdfs:domain 	mto:Device, mto:Component;
			rdfs:range 		rdfs:Literal;
			rdfs:comment 	"A unique identifier that will only refer to this device.".	

mto:hasxMotion	
			rdf:type 		owl:DatatypeProperty;
			rdfs:domain 	mto:DataItem;
			rdfs:range 		rdfs:Literal.

mto:hasxUnit	
			rdf:type 		owl:DatatypeProperty;
			rdfs:domain 	mto:DataItem;
			rdfs:range 		rdfs:Literal.


